@prefix : <http://linked.data.gov.au/def/longspine#> .
@prefix dc: <http://purl.org/dc/elements/1.1/> .
@prefix dct: <http://purl.org/dc/terms/> .
@prefix org: <http://www.w3.org/ns/org#> .
@prefix owl: <http://www.w3.org/2002/07/owl#> .
@prefix rdf: <http://www.w3.org/1999/02/22-rdf-syntax-ns#> .
@prefix sdo: <https://schema.org/> .
@prefix xml: <http://www.w3.org/XML/1998/namespace> .
@prefix xsd: <http://www.w3.org/2001/XMLSchema#> .
@prefix dcat: <http://www.w3.org/ns/dcat#> .
@prefix long: <http://linked.data.gov.au/def/longspine#> .
@prefix prov: <http://www.w3.org/ns/prov#Agent> .
@prefix rdfs: <http://www.w3.org/2000/01/rdf-schema#> .
@prefix skos: <http://www.w3.org/2004/02/skos/core#> .
@prefix time: <http://www.w3.org/2006/time> .
@base <http://linked.data.gov.au/def/longspine> .

<http://linked.data.gov.au/def/longspine> rdf:type owl:Ontology ;
                                           owl:versionIRI long: ;
                                           owl:imports skos: ,
                                                       <http://www.w3.org/2006/time> ,
                                                       org: ;
                                           dct:created "2019-06-27"^^xsd:date ;
                                           dct:creator [ sdo:email "nicholas.car@csiro.au" ;
                                                         sdo:identifier <http://orcid.org/0000-0002-8742-7730> ;
                                                         sdo:memberOf [ sdo:identifier <http://catalogue.linked.data.gov.au/org/csiro> ;
                                                                        sdo:name "CSIRO"
                                                                      ] ;
                                                         sdo:name "Nicholas J. Car"
                                                       ] ;
                                           dct:modified "2019-06-27"^^xsd:date ;
                                           dct:publisher [ sdo:identifier <http://catalogue.linked.data.gov.au/org/csiro> ;
                                                           sdo:name "CSIRO"
                                                         ] ;
                                           dct:title "LongSpine Overarching Ontology" ;
                                           rdfs:comment """An abstract model of the Longitidunal Spine of Government Functions project's main content.

This [Web Ontology Language (OWL)](https://www.w3.org/2001/sw/wiki/OWL) model is a high-level (abstract or 'upper') model that describes the general classes of object and relations between them that all [LongSpine](https://longspine.cat) *Datasets* implement.

This model declares ony a couple of its own classes and properties and inherits most of its content from existing, well-known and models, such as [Thge Organization Ontololgy](https://www.w3.org/TR/vocab-org/)."""@en ;
                                           rdfs:seeAlso "The GitHub repository containing addition documentation for this ontology is: http://github.com/CSIRO-enviro-informatics/longspine-ont"@en .

#################################################################
#    Annotation properties
#################################################################

###  http://purl.org/dc/terms/publisher
dct:publisher rdf:type owl:AnnotationProperty .


###  https://schema.org/email
sdo:email rdf:type owl:AnnotationProperty .


###  https://schema.org/identifier
sdo:identifier rdf:type owl:AnnotationProperty .


###  https://schema.org/memberOf
sdo:memberOf rdf:type owl:AnnotationProperty .


###  https://schema.org/name
sdo:name rdf:type owl:AnnotationProperty .


#################################################################
#    Object Properties
#################################################################

###  http://linked.data.gov.au/def/longspine#assigned
long:assigned rdf:type owl:ObjectProperty ;
              owl:inverseOf long:assignedTo ;
              rdf:type owl:TransitiveProperty ;
              rdfs:domain long:GovernmentStructuralUnit ;
              dct:title "assigned" ;
              skos:definition "To select for a duty" ;
              skos:scopeNote "Government Structural Units are assigned Government Functions"@en .


###  http://linked.data.gov.au/def/longspine#assignedTo
long:assignedTo rdf:type owl:ObjectProperty ,
                         owl:TransitiveProperty ;
                rdfs:range long:GovernmentStructuralUnit ;
                dct:title "assignedTo" ;
                skos:definition "To select for a duty" ;
                skos:scopeNote "Government Functions are assigned to Government Structural Units"@en .


#################################################################
#    Classes
#################################################################

###  http://linked.data.gov.au/def/longspine#Assignment
long:Assignment rdf:type owl:Class ;
                dct:title "Assignment" ;
                skos:definition "A temporally-scoped selection for duty."@en ;
                skos:scopeNote "This class is to be used when the assignment of a GovernmentFunction to a GovernmentStructuralUnit needs to be scoped temporally. If temporality in the assignment is not required (i.e. it is an eternal or timeless assignment or the temporaility is unknown) then the direct property assignedTo should be used between the GovernmentFunction and the GovernmentStructuralUnit or assigned to the invers."@en .


###  http://linked.data.gov.au/def/longspine#GovernmentFunction
long:GovernmentFunction rdf:type owl:Class ;
                        rdfs:subClassOf dcat:Role ;
                        dct:title "Government Function" ;
                        skos:definition "A function performed by a Government Structural Unit to carry out the role assigned to it."@en .


###  http://linked.data.gov.au/def/longspine#GovernmentStructuralUnit
long:GovernmentStructuralUnit rdf:type owl:Class ;
                              rdfs:subClassOf prov:Agent ;
                              dct:title "Government Structural Unit" ;
                              skos:definition "A unit of government, of any size and carrying any form of authority."@en .


###  http://www.w3.org/2006/timeTemporalEntity
time:TemporalEntity rdf:type owl:Class ;
                    skos:altLabel "Epoch" ,
                                  "Era" ;
                    skos:definition "A particular period of time marked by distinctive features, events." ;
                    skos:scopeNote "This is the Time Ontology in OWL's TemporalEntity class but is presented here with alternate labels (Epoch, Era) to allow for the use of common time period naming terms."@en .


###  http://www.w3.org/ns/dcat#Role
dcat:Role rdf:type owl:Class .


###  http://www.w3.org/ns/prov#AgentAgent
prov:Agent rdf:type owl:Class .


[ sdo:email "nicholas.car@csiro.au" ;
  sdo:identifier <http://orcid.org/0000-0002-8742-7730> ;
  sdo:memberOf [ sdo:identifier <http://catalogue.linked.data.gov.au/org/csiro> ;
                 sdo:name "CSIRO"
               ] ;
  sdo:name "Nicholas J. Car"
] .

[ sdo:identifier <http://catalogue.linked.data.gov.au/org/csiro> ;
   sdo:name "CSIRO"
 ] .

###  Generated by the OWL API (version 4.5.9.2019-02-01T07:24:44Z) https://github.com/owlcs/owlapi
